\documentclass[12pt]{article}

% Packages
\usepackage[a4paper,left=2cm,right=2cm,top=3cm,bottom=3cm]{geometry}
\usepackage{mathpazo}
\usepackage[utf8]{inputenc}
\usepackage[english]{babel}
\usepackage{amsmath,amssymb}
\usepackage{mathrsfs}

\usepackage{footnote}
\makesavenoteenv{tabular}

\setlength{\parindent}{0mm}
\def\arraystretch{1.5}

\begin{document}
\centering

{\large\bf Kernel 0}\\
\rule{0.75\textwidth}{1pt}
\begin{align}
\begin{split}
 \Delta_\sigma(E_\star,E) &= \frac{1}{\sqrt{2\pi}\sigma Z}\exp\left(\frac{-(E-E_\star)^2}{2\sigma^2}\right) \\[5mm]
 Z &= \frac{1}{2}\left(1+\mathrm{erf}\left(\frac{E_\star}{\sqrt{2}\sigma}\right)\right)
\end{split} 
\end{align}

\vskip  15mm
{\large\bf Kernel 1}\\
\rule{0.75\textwidth}{1pt}
\begin{equation}
 \Delta_\sigma(E_\star,E) = \frac{1}{\pi(E_\star-E)}\sin\left(\frac{\pi(E_\star-E)}{\sigma}\right)
\end{equation}

\vskip  15mm
{\large\bf Kernel 2}\\
\rule{0.75\textwidth}{1pt}
\begin{equation}
 \Delta_\sigma(E_\star,E) = \frac{\sigma}{(E_\star-E)^2+\sigma^2}~.
\end{equation}

\vskip  15mm
{\large\bf Kernel 3}\\
\rule{0.75\textwidth}{1pt}
\begin{equation}
 \Delta_\sigma(E_\star,E) = \frac{E_\star-E}{(E_\star-E)^2+\sigma^2}~.
\end{equation}

\pagestyle{empty}

\end{document}
